incorporate definitions from Laurent Thery's experiment

cube_explore.v
@@ -1,8 +1,494 @@
-Require Import List ZArith.
-
+Require Import List ZArith Uint63 String.
 Require Import bfs db.
 
-Check bfs.
+Import ListNotations.
 
-Definition bfs step : list (Z * Z) -> option (Zot.t Z) :=
-  fun l => bfs _ _ _ bfs_find bfs_add step 21 l empty.
+Module int_as_OT <: Structures.OrderedTypeEx.UsualOrderedType.
+
+Definition t := int.
+
+Definition lt (x y : t) := (to_Z x < to_Z y)%Z.
+
+Definition eq := @Logic.eq t.
+
+Definition eq_refl := @Logic.eq_refl t.
+
+Definition eq_sym := @Logic.eq_sym t.
+
+Definition eq_trans := @Logic.eq_trans t.
+
+Lemma lt_trans : forall x y z : t, lt x y -> lt y z -> lt x z.
+Proof.
+intros x y z; apply Z.lt_trans.
+Qed.
+
+Lemma lt_not_eq : forall x y : t, lt x y -> x <> y.
+Proof.
+intros x y xlty xy.
+rewrite xy in xlty.
+now apply Z.lt_irrefl in xlty.
+Qed.
+
+Definition compare (x y : t) : OrderedType.Compare lt eq x y.
+destruct (to_Z x ?= to_Z y)%Z eqn:cmp.  
+- apply OrderedType.EQ.
+  apply Z.compare_eq in cmp.
+  now rewrite <- (of_to_Z x), <- (of_to_Z y), cmp.
+- apply OrderedType.LT.
+  unfold lt.
+  now rewrite <- Z.compare_lt_iff.
+- apply OrderedType.GT.
+  unfold lt.
+  now rewrite <- Z.compare_gt_iff.
+Defined.
+
+Lemma eq_dec : forall x y : t, {x = y}+{x <> y}.
+Proof.
+intros x y; case (Z.eq_dec (to_Z x) (to_Z y)); intros cmp.
+- left.   
+  now rewrite <- (of_to_Z x), <- (of_to_Z y), cmp.
+- right.
+  intros xy.
+  now case cmp; rewrite xy.
+Qed.
+
+End int_as_OT.
+
+Locate Make.
+Module intmap := FMapAVL.Make int_as_OT.
+
+Arguments intmap.find _ (_)%uint63 _.
+Arguments intmap.add _ (_)%uint63 _ _.
+
+Definition empty : intmap.t Z := intmap.empty _.
+
+Definition bfs_find : intmap.t Z -> int -> option Z :=
+  fun m k => intmap.find k m.
+
+Definition bfs_add : intmap.t Z -> int -> Z -> intmap.t Z :=
+  fun m k v => intmap.add k v m.
+
+(* The following code is taken from Laurent Thery : puzzle_cube repository *)
+
+Open Scope uint63_scope.
+
+(* The number of bits for the board *)
+Definition size_board := 4.
+Definition nsize_board := 4%nat.
+Definition size_board2 := size_board * size_board.
+
+(* The number of bits for the position *)
+Definition size_position := 4.
+Definition size_board2_position := size_board2 + size_position.
+
+(* Tne number of bits for the cube *)
+Definition size_cube := 6.
+Definition size_all := size_cube + size_board2_position.
+
+Definition mask_all := (1 << size_all) -1.
+
+Definition mask_board := (1 << size_board2) -1.
+Definition clean_board := mask_all lxor mask_board.
+Definition get_board s := (s land mask_board).
+Definition set_board s i := (s land clean_board) lor i.
+
+Fixpoint mk_string n s :=
+  match n with 0 => ""%string | S n1 => append s (mk_string n1 s) end.
+
+Fixpoint print_line s n :=
+  match n with 
+  | 0 => ""%string  
+  | S n1 => if (is_zero (s land 1)) then
+              append " "%string (print_line (s >> 1) n1) 
+            else
+              append "X"%string (print_line (s >> 1) n1) 
+    end.
+
+Definition string_return := "
+"%string.
+
+Fixpoint print_board_rec s n :=
+  match n with 
+  | 0 => ""%string  
+  | S n1 => append "|"%string
+             (append (append (print_line s nsize_board) "|"%string)
+                     (append string_return
+                        (print_board_rec (s >> size_board) n1)))
+    end.
+
+Definition print_board b := 
+  append string_return (print_board_rec b nsize_board).
+
+(* Test *)
+Compute (print_board 34).
+Compute (print_board (get_board (set_board mask_all 9))).
+
+Definition mask_position := (((1 << size_position) - 1) << size_board2).
+Definition clean_position := mask_all lxor mask_position.
+Definition get_position s := (s land mask_position) >> size_board2.
+Definition get_positionX s :=
+  (get_position s) land ((1 << (size_position / 2)) - 1).
+Definition get_positionY s := (get_position s) >> (size_position / 2).
+Definition set_position s i := (s land clean_position) lor (i << size_board2).
+Definition set_positionXY s x y := 
+  set_position s ((y << (size_position / 2)) lor x).
+
+(* Lazyness : only till 9  *)
+Definition print_one_position p :=
+ if p =? 0 then "0"%string else
+ if p =? 1 then "1"%string else
+ if p =? 2 then "2"%string else
+ if p =? 3 then "3"%string else
+ if p =? 4 then "4"%string else
+ if p =? 5 then "5"%string else
+ if p =? 6 then "6"%string else
+ if p =? 7 then "7"%string else
+ if p =? 8 then "8"%string else
+ if p =? 9 then "9"%string else "?"%string.
+
+Definition print_position p :=
+  append (print_one_position (p land ((1 << (size_position / 2)) - 1)))
+  (append ", " (print_one_position (p >> (size_position / 2)))).
+
+(* Test *)
+Compute let s := set_positionXY mask_all 2 1 in
+      (print_position (get_position s)).
+
+Definition mask_cube := (((1 << size_cube) - 1) << size_board2_position).
+Definition clean_cube := mask_all lxor mask_cube.
+Definition get_cube s := (s land mask_cube) >> size_board2_position.
+Definition set_cube s i := (s land clean_cube) lor (i << size_board2_position).
+
+(* Test *)
+Compute get_cube (set_cube mask_all 12).
+
+
+(* Cube
+       ---
+       |4|
+     -------
+     |2|1|5|
+     -------
+       |3|
+       ---
+       |6|
+       ---       
+*)
+
+
+
+(* Definition d1 := 1 << 5. *)
+Definition get_d1 c := (c >> 5) land 1.
+(* Definition d2 := 1 << 4. *)
+Definition get_d2 c := (c >> 4) land 1.
+(* Definition d3 := 1 << 3. *)
+Definition get_d3 c := (c >> 3) land 1.
+(* Definition d4 := 1 << 2. *)
+Definition get_d4 c := (c >> 2) land 1.
+(* Definition d5 := 1 << 1. *)
+Definition get_d5 c := (c >> 1) land 1.
+(* Definition d6 := 1. *)
+Definition get_d6 c := c land 1.
+Definition mk_cube v1 v2 v3 v4 v5 v6 :=
+  (((((((v1 << 1 lor v2) << 1) lor v3) << 1) lor v4) << 1) lor v5) << 1 lor v6.
+
+Definition print_cube c :=
+  let f x := if is_zero x then "O"%string else "X"%string in
+  let res1 := append "         "%string 
+                (append (f (get_d4 c)) string_return) in 
+  let res2 := append "        "%string 
+                (append 
+                  (append (f (get_d2 c))(append (f (get_d1 c)) (f (get_d5 c))))
+                   string_return) in
+   let res3 := append "         "%string 
+                (append (f (get_d3 c)) string_return) in 
+   let res4 := append "         "%string 
+                (append (f (get_d6 c)) string_return) in 
+   let res5 := string_return in 
+   append (append (append (append (append
+      string_return res1) res2) res3) res4) res5. 
+
+Compute print_cube (mask_cube >> size_board2_position).
+
+(* Test *)
+Compute let c := mk_cube 0 1 0 1 0 1 in
+  (get_d1 c, get_d2 c, get_d3 c, get_d4 c, get_d5 c, get_d6 c). 
+
+(* Rol Up 
+       ---
+       |6|
+     -------
+     |2|4|5|
+     -------
+       |1|
+       ---
+       |3|
+       ---       
+
+*)
+
+Definition roll_up c :=
+  mk_cube (get_d4 c) (get_d2 c) (get_d1 c) (get_d6 c) (get_d5 c) (get_d3 c).
+
+(* Down
+       ---
+       |1|
+     -------
+     |2|3|5|
+     -------
+       |6|
+       ---
+       |4|
+       ---       
+*)
+
+Definition roll_down c :=
+  mk_cube (get_d3 c) (get_d2 c) (get_d6 c) (get_d1 c) (get_d5 c) (get_d4 c).
+
+(* Test *)
+Compute print_cube 13.
+Compute print_cube (roll_down 13).
+Compute print_cube (roll_up (roll_down 13)).
+Compute print_cube (roll_up (roll_up (roll_up (roll_up 13)))).
+
+(* Right
+       ---
+       |4|
+     -------
+     |1|5|6|
+     -------
+       |3|
+       ---
+       |2|
+       ---       
+*)
+
+Definition roll_right c :=
+  mk_cube (get_d5 c) (get_d1 c) (get_d3 c) (get_d4 c) (get_d6 c) (get_d2 c).
+
+(* Left
+       ---
+       |4|
+     -------
+     |6|2|1|
+     -------
+       |3|
+       ---
+       |5|
+       ---       
+*)
+
+Definition roll_left c :=
+  mk_cube (get_d2 c) (get_d6 c) (get_d3 c) (get_d4 c) (get_d1 c) (get_d5 c).
+
+
+(* Test *)
+Compute print_cube 13.
+Compute print_cube (roll_left 13).
+Compute print_cube (roll_left (roll_right 13)).
+Compute print_cube (roll_right (roll_right (roll_right (roll_right 13)))).
+
+Fixpoint in_state s1 l := 
+  match l with 
+  | nil => false 
+  | s2 :: l1 => if s2 <=? s1 then (s1 =? s2) else in_state s1 l1
+  end.
+
+Fixpoint add_state s1 l := 
+  match l with 
+  | nil => s1 :: nil 
+  | s2 :: l1 => if s2 <=? s1 then 
+                  if (s1 =? s2) then l else s1 :: l1 
+                  else s2 :: add_state s1 l1
+  end.
+
+Compute (add_state 11 (add_state 10 (add_state 11 nil))).
+
+Definition swap_state s := 
+  let c := get_cube s in
+  let b := get_board s in 
+  let p := get_position s in 
+  let d1 := get_d1 c in 
+  let v := (b >> p) land 1 in 
+  let s1 := set_cube s
+    (mk_cube v (get_d2 c) (get_d3 c) (get_d4 c) (get_d5 c) (get_d6 c)) in 
+  let b1 := if (v =? d1) then b else
+              if is_zero v then b lor (1 << p) else b lxor (1 << p) in
+  set_board s1 b1.
+
+Definition s0 := set_cube (set_positionXY 0 1 2) ((1 << size_cube) - 1).
+
+Compute print_cube (get_cube (swap_state s0)).
+Compute print_board (get_board (swap_state s0)).
+
+Definition one_step s vls := 
+  let px := get_positionX s in 
+  let py := get_positionY s in
+  let c := get_cube s in 
+  let (r1,vls1) := if is_zero px then (nil, vls) else
+      let c1 := roll_left c in 
+      let s1 := swap_state (set_cube (set_positionXY s (px - 1) py) c1) in
+      if in_state s1 vls then (nil, vls) else
+      (s1 :: nil, add_state s1 vls) in
+  let (r2,vls2) := if px =? (size_board - 1) then (r1, vls1) else
+      let c1 := roll_right c in 
+      let s1 := swap_state (set_cube (set_positionXY s (px + 1) py) c1) in
+      if in_state s1 vls1 then (r1, vls1) else
+      (s1 :: r1, add_state s1 vls1) in
+  let (r3,vls3) := if is_zero py then (r2, vls2) else
+      let c1 := roll_up c in 
+      let s1 := swap_state (set_cube (set_positionXY s px (py - 1)) c1) in
+      if in_state s1 vls2 then (r2, vls2) else
+      (s1 :: r2, add_state s1 vls2) in
+  let (r4,vls4) := if py =? (size_board - 1) then (r3, vls3) else
+      let c1 := roll_down c in 
+      let s1 := swap_state (set_cube (set_positionXY s px (py + 1)) c1) in
+      if in_state s1 vls3 then (r3, vls3) else
+      (s1 :: r3, add_state s1 vls3) in
+  (r4, vls4).
+
+Definition compute_state_up s : option int :=
+  let py := get_positionY s in
+  if py =? 0 then None
+  else 
+    let px := get_positionX s in
+    let s1 := set_positionXY s px (py - 1) in
+    let c := get_cube s in
+    let c1 := roll_up c in
+    let s2 := set_cube s1 c1 in
+     Some (swap_state s2).
+
+Definition compute_state_down s : option int :=
+  let py := get_positionY s in
+  if py =? size_board - 1 then None
+  else 
+    let px := get_positionX s in
+    let s1 := set_positionXY s px (py + 1) in
+    let c := get_cube s in
+    let c1 := roll_down c in
+    let s2 := set_cube s1 c1 in
+     Some (swap_state s2).
+
+Definition compute_state_left s : option int :=
+  let px := get_positionX s in
+  if px =? 0 then None
+  else 
+    let py := get_positionY s in
+    let s1 := set_positionXY s (px - 1) py in
+    let c := get_cube s in
+    let c1 := roll_up c in
+    let s2 := set_cube s1 c1 in
+     Some (swap_state s2).
+
+Definition compute_state_right s : option int :=
+  let px := get_positionX s in
+  if px =? size_board - 1 then None
+  else 
+    let py := get_positionY s in
+    let s1 := set_positionXY s (px + 1) py in
+    let c := get_cube s in
+    let c1 := roll_down c in
+    let s2 := set_cube s1 c1 in
+     Some (swap_state s2).
+
+Definition compute_pre_state_up s : list (int * Z):=
+match compute_state_up s with
+| None => nil
+| Some s1 =>
+  match compute_state_down s1 with
+  | None => nil
+  | Some s2 =>
+    match compute_state_up s2 with
+    | None => nil
+    | Some s3 => [(s3, 1%Z)]
+    end
+  end
+end.
+
+Definition compute_pre_state_right s :=
+match compute_state_right s with
+| None => nil
+| Some s1 =>
+  match compute_state_left s1 with
+  | None => nil
+  | Some s2 =>
+    match compute_state_right s2 with
+    | None => nil
+    | Some s3 => [(s3, 2%Z)]
+    end
+  end
+end.
+
+Definition compute_pre_state_down s :=
+match compute_state_down s with
+| None => nil
+| Some s1 =>
+  match compute_state_up s1 with
+  | None => nil
+  | Some s2 =>
+    match compute_state_down s2 with
+    | None => nil
+    | Some s3 => [(s3, 3%Z)]
+    end
+  end
+end.
+
+Definition compute_pre_state_left s :=
+match compute_state_left s with
+| None => nil
+| Some s1 =>
+  match compute_state_right s1 with
+  | None => nil
+  | Some s2 =>
+    match compute_state_left s2 with
+    | None => nil
+    | Some s3 => [(s3, 4%Z)]
+    end
+  end
+end.
+
+Definition reverse_steps (s : int) : list (int * Z) :=
+  compute_pre_state_left s ++
+  compute_pre_state_down s ++
+  compute_pre_state_right s ++
+  compute_pre_state_up s.
+
+Check bfs int Z (intmap.t Z) bfs_find bfs_add reverse_steps.
+
+Definition full_cube := mk_cube 1 1 1 1 1 1.
+
+Definition final_states :=
+  List.concat
+   (map (fun nx =>
+         map (fun ny => 
+           set_cube (set_positionXY 0 (of_Z (Z.of_nat nx))(of_Z (Z.of_nat ny)))
+               full_cube)
+               (seq 0 (Z.to_nat (to_Z size_board)))) 
+               (seq 0 (Z.to_nat (to_Z size_board)))).
+
+Definition print_state s := 
+    append (print_cube (get_cube s)) 
+    (append (print_position (get_position s)) (print_board (get_board s))).
+
+ Definition print_opt_state s :=
+   match s with None => ""%string | Some s => print_state s end.
+
+
+Compute get_positionY (nth 6 final_states 0).
+Compute print_position (get_position (nth 6 final_states 0)).
+
+Definition cube_explore (n : nat) : intmap.t Z + (list (int * Z) * intmap.t Z) :=
+  bfs _ _ _ bfs_find bfs_add reverse_steps n
+    (map (fun i => (i, 0%Z)) final_states) empty.
+Time Compute match cube_explore 17 with inr _ => false | inl _ => true end.
+(* answer for 17 is true in 17s *)
+Time Compute match cube_explore 16 with inr _ => false | inl _ => true end.
+(* answer for 16 is true in 17s *)
+Time Compute match cube_explore 15 with inr _ => false | inl _ => true end.
+(* answer for 15 is false in 17s *)
+Time Compute match cube_explore 14 with inl _ => 0%nat | inr (l, _) =>
+   List.length l end.
+Definition solution_map := Eval vm_compute in
+  match cube_explore 16 with inl v => v | _ => empty end.
+
+(* Amazingly this definition takes a very long time to make. *)
